code/ecdsap256/Hacl.Impl.P256.Finv.fst
@@ -8,20 +8,21 @@ module ST = FStar.HyperStack.ST
 open Lib.IntTypes
 open Lib.Buffer
 
-open Hacl.Spec.P256.MontgomeryMultiplication
-
 open Hacl.Impl.P256.Bignum
 open Hacl.Impl.P256.Field
 open Hacl.Impl.P256.Core
 open Hacl.Impl.P256.SolinasReduction
 
 module LSeq = Lib.Sequence
+
 module M = Lib.NatMod
 module LE = Lib.Exponentiation
 module SE = Spec.Exponentiation
 module BE = Hacl.Impl.Exponentiation
-module SI = Hacl.Spec.P256.Finv
+
 module S = Spec.P256
+//module SM = Hacl.Spec.P256.MontgomeryMultiplication
+module SI = Hacl.Spec.P256.Finv
 
 #reset-options "--z3rlimit 50 --fuel 0 --ifuel 0"
 
