code/ecdsap256/Hacl.Impl.P256.Finv.fsti
@@ -8,12 +8,10 @@ module ST = FStar.HyperStack.ST
 open Lib.IntTypes
 open Lib.Buffer
 
-open Spec.P256
-open Hacl.Spec.P256.MontgomeryMultiplication
 open Hacl.Spec.P256.Felem
 
-module M = Lib.NatMod
 module S = Spec.P256
+module SM = Hacl.Spec.P256.MontgomeryMultiplication
 
 #set-options "--z3rlimit 30 --fuel 0 --ifuel 0"
 
@@ -23,11 +21,13 @@ val finv: a:felem -> res:felem -> Stack unit
     as_nat h a < S.prime)
   (ensures fun h0 _ h1 -> modifies (loc res) h0 h1 /\
     as_nat h1 res < S.prime /\
-    as_nat h1 res = toDomain_ (S.finv (fromDomain_ (as_nat h0 a))))
+    as_nat h1 res = SM.toDomain_ (S.finv (SM.fromDomain_ (as_nat h0 a))))
 
 
 val fsqrt: a:felem -> res:felem -> Stack unit
-  (requires fun h -> live h a /\ live h res /\ as_nat h a < S.prime)
+  (requires fun h ->
+    live h a /\ live h res /\ disjoint a res /\
+    as_nat h a < S.prime)
   (ensures fun h0 _ h1 -> modifies (loc res) h0 h1 /\
     as_nat h1 res < S.prime /\
-    as_nat h1 res = toDomain_ (S.fsqrt (fromDomain_ (as_nat h0 a))))
+    as_nat h1 res = SM.toDomain_ (S.fsqrt (SM.fromDomain_ (as_nat h0 a))))
